src/Normal/Subst.v
@@ -28,35 +28,42 @@ Section Subst.
 
 Context `{Env}.
 
-Definition arr_equiv {dom cod} (x y : Arrow dom cod) : Type :=
+Definition rev_arr_equiv {cod dom} (x y : RevArrow cod dom) : Type :=
   arr x = arr y.
-Arguments arr_equiv {dom cod} x y.
+Arguments rev_arr_equiv {cod dom} x y.
 
-Program Instance arr_equivalence {i j} : Equivalence (@arr_equiv i j).
+Program Instance rev_arr_equivalence {j i} :
+  Equivalence (@rev_arr_equiv j i).
 Next Obligation.
-  unfold arr_equiv.
+  unfold rev_arr_equiv.
   repeat intro.
   now symmetry.
 Qed.
 Next Obligation.
-  unfold arr_equiv.
+  unfold rev_arr_equiv.
   repeat intro.
   now transitivity (arr y).
 Qed.
 
-Program Instance arr_equiv_dec {i j} :
-  EquivDec (B:=Arrow) (i:=i) (j:=j) (@arr_equiv i j)
-           (H:=@arr_equivalence i j).
+Program Instance rev_arr_Setoid {i j} : Setoid (RevArrow i j) := {
+  equiv := rev_arr_equiv;
+  setoid_equiv := rev_arr_equivalence
+}.
+
+Program Instance rev_arr_equiv_dec {j i} :
+  EquivDec (B:=RevArrow) (H:=@rev_arr_Setoid j i).
 Next Obligation.
-  unfold CEquivalence.equiv, arr_equiv, complement.
+  unfold CEquivalence.equiv, rev_arr_equiv, complement.
   destruct x, y; simpl.
-  destruct (EqDec.eq_dec arr arr0); auto.
+  destruct (EqDec.eq_dec arr arr0); subst; auto.
+    exact (Some eq_refl).
+  exact None.
 Defined.
 
-Lemma arr_eqb_equiv {dom cod} (f g : Arrow dom cod) :
-  arr_equiv f g -> mor f ≈ mor g.
+Lemma rev_arr_eqb_equiv {cod dom} (f g : RevArrow cod dom) :
+  rev_arr_equiv f g -> mor f ≈ mor g.
 Proof.
-  unfold arr_equiv; intros.
+  unfold rev_arr_equiv; intros.
   induction f, g; simpl in *.
   subst.
   rewrite present in present0.
@@ -65,25 +72,85 @@ Proof.
   now subst.
 Qed.
 
-Lemma rewrite_arrows {dom cod} :
-  ∀ f f' (Hf : termD dom cod f = Some f')
-    g g' (Hg : termD dom cod g = Some g'),
-  termD_ArrowList Hf ≈ termD_ArrowList Hg ->
-  termD dom cod f ≈ termD dom cod g.
+Lemma option_map_Proper `{Setoid A} `{Setoid B} (f : A -> B) :
+  Proper (equiv ==> equiv) f ->
+  Proper (equiv ==> equiv) (option_map f).
+Proof. proper; destruct x, y; simpl; auto. Defined.
+
+Lemma getArrMorph_Proper {dom cod} :
+  Proper (tlist_equiv (B:=RevArrow) (@rev_arr_Setoid) ==> equiv)
+         (@getArrMorph _ dom cod).
+Proof.
+  proper.
+  induction x; dependent elimination y; simpl.
+  - cat.
+  - inversion X.
+  - inversion X.
+  - simpl in X.
+    unfold TList.tlist_equiv_obligation_1 in X.
+    destruct (EqDec.eq_dec j0 j); [|contradiction].
+    subst.
+    destruct X.
+    rewrite (IHx xs).
+      comp_right.
+      now apply rev_arr_eqb_equiv.
+    exact t.
+Defined.
+
+Definition ArrowList_find
+           {j k : obj_idx} (sub : ArrowList j k)
+           {i l : obj_idx} (big : ArrowList i l) :
+  option (ArrowList k l * ArrowList i j) :=
+  tlist_find_wlist (B:=RevArrow)
+                   (@rev_arr_Setoid)
+                   (@rev_arr_equiv_dec)
+                   (i:=l) (j:=k) (k:=j) (l:=i) sub big.
+
+Definition ArrowList_find_app
+           {j k : obj_idx} (sub : ArrowList j k)
+           {i l : obj_idx} (big : ArrowList i l) {pre post} :
+  ArrowList_find sub big = Some (pre, post)
+      -> tlist_equiv (@rev_arr_Setoid) big (pre +++ sub +++ post) :=
+  fun H =>
+    tlist_find_wlist_app (B:=RevArrow)
+                         (@rev_arr_Setoid)
+                         (@rev_arr_equiv_dec)
+                         (i:=l) (j:=k) (k:=j) (l:=i)
+                         sub big H.
+
+(** The job of [rewrite_arrows] is, given two arrows being compared for
+equivalence, and another pair of equivalent arrows, and a witness to the fact
+that the first of the second pair is somewhere within the first arrow of the
+first pair, we can rewrite a goal state in terms of denoted terms into a goal
+comparing arrowlists after the rewrite has been applied. *)
+
+Lemma rewrite_arrows {dom cod} {f f' g g' i j h h' k k' a b} :
+  ∀ (Hf : termD dom cod f = Some f')
+    (Hg : termD dom cod g = Some g')
+    (Hh : termD i j h = Some h')
+    (Hk : termD i j k = Some k'),
+    let fs := `1 (Term_to_ArrowList_sound Hf) in
+    let gs := `1 (Term_to_ArrowList_sound Hg) in
+    let hs := `1 (Term_to_ArrowList_sound Hh) in
+    ArrowList_find hs fs = Some (a, b)
+      -> a +++ hs +++ b ≈ gs
+      -> termD dom cod f ≈ termD dom cod g.
 Proof.
   intros.
   rewrite !termD_getMorph_fromTerm.
-  destruct (fromTerm dom cod f) eqn:?,
-           (fromTerm dom cod g) eqn:?.
-  simpl.
-  admit.
-  rewrite !getMorph_getArrMorph.
-  red.
-  rewrite Hf, Hg.
-  f_equiv.
-  red in X.
-  (* jww (2018-03-08): Need a way to turn termD = Some into a ValidTerm,
-     and then from there go to an ArrowList. *)
-Abort.
+  remember (Term_to_ArrowList_sound Hf) as HHf; destruct HHf.
+  remember (Term_to_ArrowList_sound Hg) as HHg; destruct HHg.
+  remember (Term_to_ArrowList_sound Hh) as HHh; destruct HHh.
+  rewrite e, e0; simpl.
+  unfold fs in *; clear fs.
+  unfold gs in *; clear gs.
+  unfold hs in *; clear hs.
+  simpl in *.
+  pose proof (ArrowList_find_app x1 x (pre:=a) (post:=b) H0).
+  apply getArrMorph_Proper in X0.
+  now rewrite X0.
+Defined.
+
+Print Assumptions rewrite_arrows.
 
 End Subst.
