src/Normal/Valid.v
@@ -6,6 +6,7 @@ Require Import Coq.Lists.List.
 Require Import Coq.omega.Omega.
 
 Require Import Equations.Equations.
+Require Import Equations.EqDec.
 Unset Equations WithK.
 
 Require Import Category.Lib.
@@ -14,6 +15,7 @@ Require Import Category.Theory.Category.
 Require Import Solver.Lib.
 Require Import Solver.Env.
 Require Import Solver.Expr.Term.
+Require Import Solver.Expr.Denote.
 Require Import Solver.Normal.TList.
 Require Import Solver.Normal.Arrow.
 Require Import Solver.Normal.Denote.
@@ -23,6 +25,231 @@ Generalizable All Variables.
 Section NormalValid.
 
 Context `{H : Env}.
+
+Import EqNotations.
+
+Equations getArrMorph {dom cod} (a : ArrowList dom cod) :
+  objs dom ~> objs cod :=
+  getArrMorph tnil := id;
+  getArrMorph (tcons f g) := mor f ∘ getArrMorph g.
+
+Lemma getArrMorph_ArrowList_compose {dom mid cod}
+      (f : ArrowList mid cod)
+      (g : ArrowList dom mid) :
+  getArrMorph (f +++ g) ≈ getArrMorph f ∘ getArrMorph g.
+Proof.
+  induction f.
+    rewrite getArrMorph_equation_1; cat.
+  rewrite <- tlist_app_comm_cons.
+  rewrite !getArrMorph_equation_2.
+  now rewrite IHf; cat.
+Qed.
+
+Program Definition option_dec {A} (x : option A) :
+  (∃ y : A, x = Some y) + (x = None) :=
+  match x with
+  | Some y => inl (y; _)
+  | None => inr _
+  end.
+
+Equations Term_to_ArrowList_work (dom : obj_idx) (f : Term) :
+  option (∃ cod, ArrowList dom cod) :=
+  Term_to_ArrowList_work dom Identity := Some (dom; tnil);
+  Term_to_ArrowList_work dom (Morph a) <= option_dec (arrs a) => {
+    | inl (existT (existT dom' (existT cod f')) Hf')
+      <= eq_dec dom dom' => {
+        | left H =>
+          Some (cod; Build_Arrow dom cod a
+                  (rew <- [fun x => objs x ~> _] H in f') _ ::: tnil);
+        | _ => None
+      };
+    | inr _ => None
+  };
+  Term_to_ArrowList_work dom (Compose f g)
+    <= Term_to_ArrowList_work dom g => {
+      | Some (existT mid u) <= Term_to_ArrowList_work mid f => {
+          | Some (existT cod t) =>
+            Some (cod; t +++ u);
+          | None => None
+        };
+      | None => None
+    }.
+
+Definition Term_to_ArrowList dom cod (f : Term) : option (ArrowList dom cod) :=
+  match Term_to_ArrowList_work dom f with
+  | Some (y; v) =>
+    match Eq_eq_dec y cod with
+    | left H => Some (rew [fun y => ArrowList dom y] H in v)
+    | _ => None
+    end
+  | _ => None
+  end.
+
+Global Program Instance mor_work_Setoid {dom} :
+  Setoid (∃ cod : obj_idx, objs dom ~> objs cod) := {
+  equiv := fun f g => match Eq_eq_dec `1 f `1 g with
+    | left H => `2 f ≈ rew <- [fun x => _ ~> objs x] H in `2 g
+    | right _ => False
+    end
+}.
+Next Obligation.
+  equivalence; simpl in *.
+  - now rewrite Pos_eq_dec_refl.
+  - destruct (Pos.eq_dec x1 x0); [|contradiction]; subst.
+    rewrite Pos_eq_dec_refl.
+    now symmetry.
+  - destruct (Pos.eq_dec x1 x0); [|contradiction]; subst.
+    destruct (Pos.eq_dec x2 x0); [|contradiction]; subst.
+    now transitivity e0.
+Qed.
+
+Lemma termD_work_getMorph_fromTerm {dom f} :
+  termD_work dom f ≈ option_map (fun '(cod; p) => (cod; getArrMorph p))
+                                (Term_to_ArrowList_work dom f).
+Proof.
+  generalize dependent dom.
+  induction f; intros.
+  - rewrite Term_to_ArrowList_work_equation_1; simpl.
+    rewrite Pos_eq_dec_refl; cat.
+  - rewrite Term_to_ArrowList_work_equation_2.
+    unfold Term_to_ArrowList_work_obligation_3.
+    unfold Term_to_ArrowList_work_obligation_2.
+    unfold Term_to_ArrowList_work_obligation_1.
+    destruct (option_dec (arrs a)).
+      destruct s, x, s; simpl.
+      dependent rewrite e.
+      unfold eq_dec.
+      destruct (Pos.eq_dec x dom).
+        subst.
+        rewrite Pos_eq_dec_refl; simpl.
+        rewrite Pos_eq_dec_refl; simpl.
+        rewrite getArrMorph_equation_2; simpl.
+        rewrite getArrMorph_equation_1; simpl.
+        simpl_eq; cat.
+      destruct (Pos.eq_dec dom x); auto.
+        subst; contradiction.
+      constructor.
+    now simpl; rewrite e.
+  - rewrite Term_to_ArrowList_work_equation_3.
+    unfold Term_to_ArrowList_work_obligation_5.
+    unfold Term_to_ArrowList_work_obligation_4.
+    specialize (IHf2 dom).
+    destruct (Term_to_ArrowList_work dom f2) eqn:?; auto.
+      destruct s.
+      simpl termD_work.
+      simpl option_map in IHf2.
+      destruct (termD_work dom f2); [|inversion IHf2]; auto.
+      destruct s.
+      specialize (IHf1 x0).
+      destruct (Term_to_ArrowList_work x0 f1) eqn:?; auto.
+        destruct s.
+        simpl option_map in IHf1.
+        destruct (termD_work x0 f1); [|inversion IHf1]; auto.
+        destruct s.
+        do 2 red in IHf1.
+        do 2 red in IHf2.
+        simpl in *.
+        destruct (Pos.eq_dec x0 x); [|contradiction].
+        destruct (Pos.eq_dec x2 x1); [|contradiction].
+        subst.
+        rewrite Heqo0.
+        simpl.
+        rewrite Pos_eq_dec_refl.
+        simpl_eq.
+        rewrite getArrMorph_ArrowList_compose.
+        now rewrite IHf1, IHf2.
+      simpl in IHf1.
+      destruct (termD_work x0 f1); [contradiction|]; auto.
+      do 2 red in IHf2.
+      simpl in *.
+      destruct (Pos.eq_dec x0 x); [|contradiction].
+      subst.
+      rewrite Heqo0; simpl; auto.
+    simpl in *.
+    destruct (termD_work dom f2); [contradiction|]; auto.
+Defined.
+
+Lemma termD_getMorph_fromTerm {dom cod f} :
+  termD dom cod f ≈ option_map getArrMorph (Term_to_ArrowList dom cod f).
+Proof.
+  unfold termD, Term_to_ArrowList.
+  pose proof (@termD_work_getMorph_fromTerm dom f).
+  red in X.
+  destruct (termD_work dom f) eqn:?.
+    destruct s.
+    destruct (Term_to_ArrowList_work dom f) eqn:?; simpl; auto.
+      destruct s.
+      simpl in X.
+      destruct (Pos.eq_dec x x0); subst; [|contradiction].
+      destruct (Pos.eq_dec x0 cod); subst.
+        exact X.
+      constructor.
+    simpl in X.
+    contradiction.
+  destruct (Term_to_ArrowList_work dom f) eqn:?; simpl; auto.
+  destruct s.
+  simpl in *.
+  contradiction.
+Defined.
+
+Lemma Term_to_ArrowList_sound {dom cod f f'} :
+  termD dom cod f = Some f'
+    -> ∃ xs, Term_to_ArrowList dom cod f = Some xs.
+Proof.
+  unfold termD, Term_to_ArrowList; intros.
+  generalize dependent cod.
+  generalize dependent dom.
+  induction f; simpl; intros.
+  - destruct (Pos.eq_dec dom cod); [|discriminate].
+    subst.
+    exists tnil.
+    rewrite Term_to_ArrowList_work_equation_1.
+    rewrite Pos_eq_dec_refl.
+    reflexivity.
+  - rewrite Term_to_ArrowList_work_equation_2.
+    unfold Term_to_ArrowList_work_obligation_3.
+    destruct (option_dec (arrs a)).
+      destruct s, x, s.
+      rewrite e in *.
+      destruct (Pos.eq_dec x dom); [|discriminate]; subst.
+      rewrite eq_dec_refl.
+      destruct (Pos.eq_dec x0 cod); [|discriminate]; subst.
+      simpl in *.
+      rewrite Pos_eq_dec_refl.
+      simpl.
+      eexists; reflexivity.
+    rewrite e in *.
+    discriminate.
+  - rewrite Term_to_ArrowList_work_equation_3.
+    unfold Term_to_ArrowList_work_obligation_5.
+    destruct (termD_work dom f2) eqn:?; [|discriminate].
+    destruct s.
+    destruct (termD_work x f1) eqn:?; [|discriminate].
+    destruct s.
+    destruct (Pos.eq_dec x0 cod); [|discriminate]; subst.
+    simpl in *.
+    specialize (IHf1 x cod h0).
+    rewrite Heqo0, Pos_eq_dec_refl in IHf1.
+    specialize (IHf1 eq_refl).
+    specialize (IHf2 dom x h).
+    rewrite Heqo, Pos_eq_dec_refl in IHf2.
+    specialize (IHf2 eq_refl).
+    simpl in *.
+    destruct IHf1 as [xs ?].
+    destruct IHf2 as [ys ?].
+    exists (xs +++ ys).
+    destruct (Term_to_ArrowList_work dom f2); [|discriminate].
+    destruct s; simpl.
+    destruct (Pos.eq_dec x0 x); [|discriminate]; subst.
+    unfold Term_to_ArrowList_work_obligation_4.
+    destruct (Term_to_ArrowList_work x f1); [|discriminate].
+    destruct s.
+    destruct (Pos.eq_dec x0 cod); [|discriminate]; subst.
+    simpl in *.
+    inversion e; subst.
+    inversion e0; subst.
+    reflexivity.
+Defined.
 
 (*
 
@@ -53,11 +280,6 @@ Next Obligation.
     pose proof wildcard18.
     apply FMapPositive.PositiveMap.elements_correct in H0.
 *)
-
-Equations getArrMorph {dom cod} (a : ArrowList dom cod) :
-  objs dom ~> objs cod :=
-  getArrMorph tnil := id;
-  getArrMorph (tcons f g) := mor f ∘ getArrMorph g.
 
 (*
 Lemma ArrowList_compose_inv {dom cod fs gs} :
@@ -153,18 +375,6 @@ Corollary ArrowList_cod_eq {dom cod}
   cod = cod'.
 Proof. intros; destruct (ArrowList_dom_cod_eq f g); auto. Qed.
 *)
-
-Lemma getArrMorph_ArrowList_compose {dom mid cod}
-      (f : ArrowList mid cod)
-      (g : ArrowList dom mid) :
-  getArrMorph (f +++ g) ≈ getArrMorph f ∘ getArrMorph g.
-Proof.
-  induction f.
-    rewrite getArrMorph_equation_1; cat.
-  rewrite <- tlist_app_comm_cons.
-  rewrite !getArrMorph_equation_2.
-  now rewrite IHf; cat.
-Qed.
 
 (*
 Equations ArrowList_eq_arr {dom cod fs}
